systems/ZTreeAggregationDynamicCorrect.v
@@ -1,0 +1,57 @@
+Require Import Verdi.Verdi.
+Require Import Verdi.HandlerMonad.
+Require Import Verdi.NameOverlay.
+
+Require Import TreeAux.
+Require Import ZTreeAggregationDynamic.
+
+Require Import Sumbool.
+Require Import Orders.
+Require Import MSetFacts.
+Require Import MSetProperties.
+
+Require Import mathcomp.ssreflect.ssreflect.
+Require Import mathcomp.ssreflect.ssrbool.
+
+Local Arguments update {_} {_} _ _ _ _ _ : simpl never.
+
+Module ZTreeAggregationCorrect (Import NT : NameType)  
+ (NOT : NameOrderedType NT) (NSet : MSetInterface.S with Module E := NOT) 
+ (NOTC : NameOrderedTypeCompat NT) (NMap : FMapInterface.S with Module E := NOTC) 
+ (Import RNT : RootNameType NT) 
+ (Import ANT : AdjacentNameType NT) 
+ (Import TA : TAux NT NOT NSet NOTC NMap).
+
+Module ZTG := ZTreeAggregation NT NOT NSet NOTC NMap RNT ANT TA.
+Import ZTG.
+
+Module NSetFacts := Facts NSet.
+Module NSetProps := Properties NSet.
+Module NSetOrdProps := OrdProperties NSet.
+
+Require Import FMapFacts.
+Module NMapFacts := Facts NMap.
+
+Definition sum_aggregate (ns : list name) (state : name -> option data) : Z :=
+fold_right (fun d z => (z + d.(aggregate))%Z) 0%Z (filterMap state ns).
+
+Definition sum_aggregate_msg := fold_right (fun m z => (z + match m with Aggregate z' => z' | _ => 0%Z end)%Z) 0%Z.
+
+Definition sum_aggregate_msg_to (ns : list name) (packets : name -> name -> list msg) (n : name) : Z :=
+fold_right (fun n' z => (z + sum_aggregate_msg (packets n' n))%Z) 0%Z ns.
+
+Definition sum_aggregate_msg_to_all (ns : list name) (packets : name -> name -> list msg) : Z :=
+fold_right (fun n z => (z + sum_aggregate_msg_to ns packets n)%Z) 0%Z ns.
+
+Definition conserves_network_mass net :=
+  Z_of_nat (length net.(odnwNodes)) = 
+  (sum_aggregate net.(odnwNodes) net.(odnwState) + sum_aggregate_msg_to_all net.(odnwNodes) net.(odnwPackets))%Z.
+
+Lemma ZTreeAggregation_conserves_network_mass :
+  forall net tr,
+    step_ordered_dynamic_star step_ordered_dynamic_init net tr ->        
+    conserves_network_mass net.
+Proof.
+Admitted.
+
+End ZTreeAggregationCorrect.
