systems/ZTreeAggregationDynamicLabeledCorrect.v
@@ -1,0 +1,51 @@
+Require Import Verdi.Verdi.
+Require Import Verdi.HandlerMonad.
+Require Import Verdi.NameOverlay.
+Require Import Verdi.LabeledNet.
+
+Require Import TreeAux.
+Require Import ZTreeAggregationDynamicLabeled.
+
+Require Import InfSeqExt.infseq.
+
+Require Import Sumbool.
+Require String.
+
+Require Import ZArith.
+
+Require Import mathcomp.ssreflect.ssreflect.
+Require Import mathcomp.ssreflect.ssrbool.
+
+Local Arguments update {_} {_} _ _ _ _ _ : simpl never.
+
+Set Implicit Arguments.
+
+Module ZTreeAggregationCorrect (Import NT : NameType)  
+ (NOT : NameOrderedType NT) (NSet : MSetInterface.S with Module E := NOT) 
+ (NOTC : NameOrderedTypeCompat NT) (NMap : FMapInterface.S with Module E := NOTC) 
+ (Import RNT : RootNameType NT) 
+ (Import ANT : AdjacentNameType NT) 
+ (Import TA : TAux NT NOT NSet NOTC NMap).
+
+Module ZTA := ZTreeAggregation NT NOT NSet NOTC NMap RNT ANT TA.
+Import ZTA.
+
+Definition connected net := net.(odnwNodes) = net.(odnwNodes). (* FIXME *)
+
+Definition node_aggregate (state : name -> option data) (n : name) : Z :=
+match state n with
+| None => 0%Z
+| Some d => d.(aggregate)
+end.
+
+Lemma churn_free_stabilization : 
+  forall s, event_step_star step_ordered_dynamic step_ordered_dynamic_init (hd s) ->
+       connected (evt_a (hd s)) ->
+       lb_step_execution lb_step_ordered_dynamic s ->
+       weak_fairness lb_step_ordered_dynamic Tau s ->
+       forall n, root n -> In n (evt_a (hd s)).(odnwNodes) ->
+       eventually (always (now (fun e => Z_of_nat (length e.(evt_a).(odnwNodes)) = node_aggregate e.(evt_a).(odnwState) n))) s.
+Proof.
+Admitted.
+
+End ZTreeAggregationCorrect.
